proving the soundness

GCSL.v
@@ -1,4 +1,5 @@
-Require Export CSL array_dist.
+Require Export CSL.
+Require Import array_dist Bdiv.
 Import PHeap Lang assertion_lemmas.
 
 Section GlobalCSL.
@@ -20,15 +21,6 @@ Definition default_stack : stack := fun x => 0%Z.
 Require Import MyVector.
 Import VectorNotations.
 
-Definition hdisj_sim (h1 h2 : simple_heap) :=
-  forall x, h1 x = None \/ h2 x = None.
-
-Definition hplus_sim (h1 h2 : simple_heap) :=
-  fun x => match h1 x with
-    | Some x => Some x
-    | None => h2 x
-  end.
-
 Definition bdiv_g (gs : g_state nblk ntrd) :=
   exists bid : Fin.t nblk, 
     Bdiv.bdiv ((blks gs)[@bid], sh_gl_heap (sh_hp gs)[@bid] (gl_hp gs)).
@@ -40,14 +32,14 @@ Fixpoint safe_ng (n : nat) (gs : g_state nblk ntrd) (Q : assn) :=
       ((forall (bid : Fin.t nblk) (tid : Fin.t ntrd), fst ((blks gs)[@bid][@tid]) = SKIP) ->
          Q default_stack (htop (heap_of_sheap (gl_hp gs)))) /\
       (forall hF : simple_heap,
-         hdisj_sim (gl_hp gs) hF ->
-         ~abort_g (Gs (blks gs) (sh_hp gs) (hplus_sim (gl_hp gs) hF))) /\
+         hdisj (gl_hp gs) hF ->
+         ~abort_g (Gs (blks gs) (sh_hp gs) (hplus (gl_hp gs) hF))) /\
       ~ bdiv_g gs /\
       (forall (gs' : g_state nblk ntrd) (hF : simple_heap),
-         hdisj_sim (gl_hp gs) hF ->
-         red_g (Gs (blks gs) (sh_hp gs) (hplus_sim (gl_hp gs) hF)) gs' ->
+         hdisj (gl_hp gs) hF ->
+         red_g (Gs (blks gs) (sh_hp gs) (hplus (gl_hp gs) hF)) gs' ->
          exists h'' : simple_heap,
-           hdisj_sim h'' hF /\ (gl_hp gs') = hplus_sim h'' hF /\
+           hdisj h'' hF /\ (gl_hp gs') = hplus h'' hF /\
            safe_ng n (Gs (blks gs') (sh_hp gs') h'') Q)
   end.
 
@@ -78,7 +70,7 @@ Section For_List_Notation.
   Fixpoint sh_spec (sh_decl : list (var * nat)) : assn :=
     match sh_decl with
       | nil => emp
-      | (sh, len) :: sh_decl => is_array (Sh sh) len (fun _ => 0%Z) 0 ** sh_spec sh_decl
+      | (sh, len) :: sh_decl => (Ex f, is_array (Sh sh) len f 0) ** sh_spec sh_decl
     end.
   
   Notation TID := (Var 0).
@@ -96,7 +88,25 @@ Section For_List_Notation.
          (forall tid bid v, v <> TID -> v <> BID -> snd ks[@bid][@tid] v = stk v) /\
          P stk (htop (heap_of_sheap gh))) ->
     forall n, safe_ng n (Gs ks (const sh nblk) gh) Q.
+
+  Definition has_no_vars (P : assn) : Prop := indeP (fun (_ _ : stack) => True) P.
   
-  Lemma safe_gl (C : cmd) (Q : assn) (Qs : Vector.t assn nblk) 
-  :
-    
+  Lemma safe_gl (n : nat) :
+    forall (gs : g_state nblk ntrd) (Q : assn) (Qs : Vector.t assn nblk),
+    (forall bid : Fin.t nblk,
+       safe_nk E n (fst (bs_of_gs gs bid)) (snd (bs_of_gs gs bid)) (sh_spec prog ** Qs[@bid])) ->
+    (forall bid : Fin.t nblk, has_no_vars Qs[@bid]) ->
+    Aistar_v (Qs |= Q) -> 
+    safe_ng n gs Q.
+  Proof.
+    induction n; simpl; auto.
+    intros gs Q Qs Hsafe Hnov HQ; repeat split.
+    - intros Hskip.
+      evar (P : Fin.t nblk -> Prop); assert (Hskipb : forall bid, P bid); [|unfold P in *; clear P].
+      { unfold P; intros bid; destruct (Hsafe bid) as (Hskipb & _).
+        apply Hskipb in Hskip as (? & ?).
+        unfold sat_k in H; simpl in H.
+        lazymatch type of H with (let (_, _) := ?X in _) => destruct X end.
+        unfold has_no_vars, indeP in Hnov; simpl in Hnov; rewrite (Hnov _ _ default_stack) in H; auto.
+        exact H. }
+      
